{
	"@context": {
		"rdf": "http://www.w3.org/1999/02/22-rdf-syntax-ns#",
		"rdfs": "http://www.w3.org/2000/01/rdf-schema#",
		"schema": "http://schema.org/",
		"iot": "http://iotschema.org/",
		"rdfs:subClassOf": {
			"@type": "@vocab"
		},
		"rdfs:seeAlso": {
			"@type": "@vocab"
		}
	},
	"@graph": [
		{
			"@id": "iot:BinarySwitchChanged",
			"@type": "rdfs:Class",
			"rdfs:subClassOf": "iot:PropertyChangedEvent",
			"rdfs:label": "BinarySwitchChanged",
			"rdfs:comment": "Specification of an event occurring when some property of type BinarySwitch changes.",
			"rdfs:seeAlso": "http://iotschema.org/BinarySwitch"
		},
		{
			"@id": "iot:CountDownChanged",
			"@type": "rdfs:Class",
			"rdfs:subClassOf": "iot:PropertyChangedEvent",
			"rdfs:label": "CountDownChanged",
			"rdfs:comment": "Specification of an event occurring when some property of type CountDown changes.",
			"rdfs:seeAlso": "http://iotschema.org/CountDown"
		},
		{
			"@id": "iot:CurrentColourChanged",
			"@type": "rdfs:Class",
			"rdfs:subClassOf": "iot:PropertyChangedEvent",
			"rdfs:label": "CurrentColourChanged",
			"rdfs:comment": "Specification of an event occurring when some property of type CurrentColour changes.",
			"rdfs:seeAlso": "http://iotschema.org/CurrentColour"
		},
		{
			"@id": "iot:CurrentDimmerChanged",
			"@type": "rdfs:Class",
			"rdfs:subClassOf": "iot:PropertyChangedEvent",
			"rdfs:label": "CurrentDimmerChanged",
			"rdfs:comment": "Specification of an event occurring when some property of type CurrentDimmer changes.",
			"rdfs:seeAlso": "http://iotschema.org/CurrentDimmer"
		},
		{
			"@id": "iot:CurrentLevelChanged",
			"@type": "rdfs:Class",
			"rdfs:subClassOf": "iot:PropertyChangedEvent",
			"rdfs:label": "CurrentLevelChanged",
			"rdfs:comment": "Specification of an event occurring when some property of type CurrentLevel changes.",
			"rdfs:seeAlso": "http://iotschema.org/CurrentLevel"
		},
		{
			"@id": "iot:ExpectedDensityChanged",
			"@type": "rdfs:Class",
			"rdfs:subClassOf": "iot:PropertyChangedEvent",
			"rdfs:label": "ExpectedDensityChanged",
			"rdfs:comment": "Specification of an event occurring when some property of type ExpectedDensity changes.",
			"rdfs:seeAlso": "http://iotschema.org/ExpectedDensity"
		},
		{
			"@id": "iot:ExpectedFloatImmersionDepthChanged",
			"@type": "rdfs:Class",
			"rdfs:subClassOf": "iot:PropertyChangedEvent",
			"rdfs:label": "ExpectedFloatImmersionDepthChanged",
			"rdfs:comment": "Specification of an event occurring when some property of type ExpectedFloatImmersionDepth changes.",
			"rdfs:seeAlso": "http://iotschema.org/ExpectedFloatImmersionDepth"
		},
		{
			"@id": "iot:ExpectedFlowRateChanged",
			"@type": "rdfs:Class",
			"rdfs:subClassOf": "iot:PropertyChangedEvent",
			"rdfs:label": "ExpectedFlowRateChanged",
			"rdfs:comment": "Specification of an event occurring when some property of type ExpectedFlowRate changes.",
			"rdfs:seeAlso": "http://iotschema.org/ExpectedFlowRate"
		},
		{
			"@id": "iot:ExpectedPressureChanged",
			"@type": "rdfs:Class",
			"rdfs:subClassOf": "iot:PropertyChangedEvent",
			"rdfs:label": "ExpectedPressureChanged",
			"rdfs:comment": "Specification of an event occurring when some property of type ExpectedPressure changes.",
			"rdfs:seeAlso": "http://iotschema.org/ExpectedPressure"
		},
		{
			"@id": "iot:ExpectedUpstreamPressureChanged",
			"@type": "rdfs:Class",
			"rdfs:subClassOf": "iot:PropertyChangedEvent",
			"rdfs:label": "ExpectedUpstreamPressureChanged",
			"rdfs:comment": "Specification of an event occurring when some property of type ExpectedUpstreamPressure changes.",
			"rdfs:seeAlso": "http://iotschema.org/ExpectedUpstreamPressure"
		},
		{
			"@id": "iot:HumidityChanged",
			"@type": "rdfs:Class",
			"rdfs:subClassOf": "iot:PropertyChangedEvent",
			"rdfs:label": "HumidityChanged",
			"rdfs:comment": "Specification of an event occurring when some property of type Humidity changes.",
			"rdfs:seeAlso": "http://iotschema.org/Humidity"
		},
		{
			"@id": "iot:IlluminanceChanged",
			"@type": "rdfs:Class",
			"rdfs:subClassOf": "iot:PropertyChangedEvent",
			"rdfs:label": "IlluminanceChanged",
			"rdfs:comment": "Specification of an event occurring when some property of type Illuminance changes.",
			"rdfs:seeAlso": "http://iotschema.org/Illuminance"
		},
		{
			"@id": "iot:MotionTypeChanged",
			"@type": "rdfs:Class",
			"rdfs:subClassOf": "iot:PropertyChangedEvent",
			"rdfs:label": "MotionTypeChanged",
			"rdfs:comment": "Specification of an event occurring when some property of type MotionType changes.",
			"rdfs:seeAlso": "http://iotschema.org/MotionType"
		},
		{
			"@id": "iot:OperationStatusChanged",
			"@type": "rdfs:Class",
			"rdfs:subClassOf": "iot:PropertyChangedEvent",
			"rdfs:label": "OperationStatusChanged",
			"rdfs:comment": "Specification of an event occurring when some property of type OperationStatus changes.",
			"rdfs:seeAlso": "http://iotschema.org/OperationStatus"
		},
		{
			"@id": "iot:OverflowStatusChanged",
			"@type": "rdfs:Class",
			"rdfs:subClassOf": "iot:PropertyChangedEvent",
			"rdfs:label": "OverflowStatusChanged",
			"rdfs:comment": "Specification of an event occurring when some property of type OverflowStatus changes.",
			"rdfs:seeAlso": "http://iotschema.org/OverflowStatus"
		},
		{
			"@id": "iot:RampTimeChanged",
			"@type": "rdfs:Class",
			"rdfs:subClassOf": "iot:PropertyChangedEvent",
			"rdfs:label": "RampTimeChanged",
			"rdfs:comment": "Specification of an event occurring when some property of type RampTime changes.",
			"rdfs:seeAlso": "http://iotschema.org/RampTime"
		},
		{
			"@id": "iot:RunModeChanged",
			"@type": "rdfs:Class",
			"rdfs:subClassOf": "iot:PropertyChangedEvent",
			"rdfs:label": "RunModeChanged",
			"rdfs:comment": "Specification of an event occurring when some property of type RunMode changes.",
			"rdfs:seeAlso": "http://iotschema.org/RunMode"
		},
		{
			"@id": "iot:SoundPressureLevelChanged",
			"@type": "rdfs:Class",
			"rdfs:subClassOf": "iot:PropertyChangedEvent",
			"rdfs:label": "SoundPressureLevelChanged",
			"rdfs:comment": "Specification of an event occurring when some property of type SoundPressureLevel changes.",
			"rdfs:seeAlso": "http://iotschema.org/SoundPressureLevel"
		},
		{
			"@id": "iot:SwitchStatusChanged",
			"@type": "rdfs:Class",
			"rdfs:subClassOf": "iot:PropertyChangedEvent",
			"rdfs:label": "SwitchStatusChanged",
			"rdfs:comment": "Specification of an event occurring when some property of type SwitchStatus changes.",
			"rdfs:seeAlso": "http://iotschema.org/SwitchStatus"
		},
		{
			"@id": "iot:TargetHumidityChanged",
			"@type": "rdfs:Class",
			"rdfs:subClassOf": "iot:PropertyChangedEvent",
			"rdfs:label": "TargetHumidityChanged",
			"rdfs:comment": "Specification of an event occurring when some property of type TargetHumidity changes.",
			"rdfs:seeAlso": "http://iotschema.org/TargetHumidity"
		},
		{
			"@id": "iot:TargetTemperatureChanged",
			"@type": "rdfs:Class",
			"rdfs:subClassOf": "iot:PropertyChangedEvent",
			"rdfs:label": "TargetTemperatureChanged",
			"rdfs:comment": "Specification of an event occurring when some property of type TargetTemperature changes.",
			"rdfs:seeAlso": "http://iotschema.org/TargetTemperature"
		},
		{
			"@id": "iot:TemperatureChanged",
			"@type": "rdfs:Class",
			"rdfs:subClassOf": "iot:PropertyChangedEvent",
			"rdfs:label": "TemperatureChanged",
			"rdfs:comment": "Specification of an event occurring when some property of type Temperature changes.",
			"rdfs:seeAlso": "http://iotschema.org/Temperature"
		},
		{
			"@id": "iot:TransitionTimeChanged",
			"@type": "rdfs:Class",
			"rdfs:subClassOf": "iot:PropertyChangedEvent",
			"rdfs:label": "TransitionTimeChanged",
			"rdfs:comment": "Specification of an event occurring when some property of type TransitionTime changes.",
			"rdfs:seeAlso": "http://iotschema.org/TransitionTime"
		},
		{
			"@id": "iot:WindStrengthChanged",
			"@type": "rdfs:Class",
			"rdfs:subClassOf": "iot:PropertyChangedEvent",
			"rdfs:label": "WindStrengthChanged",
			"rdfs:comment": "Specification of an event occurring when some property of type WindStrength changes.",
			"rdfs:seeAlso": "http://iotschema.org/WindStrength"
		}
	]
}